mechanization/theories/Core/Soundness/LogicalRelation/CoreLemmas.v
@@ -15,20 +15,20 @@ Ltac simpl_glu_rel :=
   destruct_all;
   gen_presups.
 
-Lemma glu_sort_elem_sort_wf_exp_sort {P} (pred_P : PredicativeSig P) : forall s typ_rel exp_rel a,
-    {{ DG a ∈ glu_sort_elem pred_P s ↘ typ_rel ↘ exp_rel }} ->
-    forall Γ A,
-      {{ Γ ⊢ A ® typ_rel }} ->
-      {{ Γ ⊢ A : Sort@s }}.
-Proof.
-  simpl.
-  induction 1 using glu_sort_elem_ind; intros;
-    simpl_glu_rel; mauto 2.
+(* Lemma glu_sort_elem_sort_wf_exp_sort {P} (pred_P : PredicativeSig P) : forall s typ_rel exp_rel a, *)
+(*     {{ DG a ∈ glu_sort_elem pred_P s ↘ typ_rel ↘ exp_rel }} -> *)
+(*     forall Γ A, *)
+(*       {{ Γ ⊢ A ® typ_rel }} -> *)
+(*       {{ Γ ⊢ A : Sort@s }}. *)
+(* Proof. *)
+(*   simpl. *)
+(*   induction 1 using glu_sort_elem_ind; intros; *)
+(*     simpl_glu_rel; mauto 2. *)
 
-  assert {{ Γ ⊢ A[Id] ≈ Sort@s' : Sort@s }} by (eapply H3; mauto 3).
-  gen_presup H4.
-  mauto 2.
-Qed.
+(*   assert {{ Γ ⊢ A[Id] ≈ Sort@s' : Sort@s }} by (eapply H3; mauto 3). *)
+(*   gen_presup H4. *)
+(*   mauto 2. *)
+(* Qed. *)
 
 Lemma glu_sort_elem_sort_lvl {P} (pred_P : PredicativeSig P) : forall s typ_rel exp_rel a,
     {{ DG a ∈ glu_sort_elem pred_P s ↘ typ_rel ↘ exp_rel }} ->
@@ -36,9 +36,9 @@ Lemma glu_sort_elem_sort_lvl {P} (pred_P : PredicativeSig P) : forall s typ_rel 
       {{ Γ ⊢ A ® typ_rel }} ->
       {{ Γ ⊢ A }}.
 Proof.
-  intros.
-  assert {{ Γ ⊢ A : Sort@s }} by (eapply glu_sort_elem_sort_wf_exp_sort; mauto 2).
-  mauto 2.
+  simpl.
+  induction 1 using glu_sort_elem_ind;
+    intros; simpl_glu_rel; mauto 2.
 Qed.
 
 Lemma glu_sort_elem_typ_resp_typ_eq {P} (pred_P : PredicativeSig P) : forall s typ_rel exp_rel a,
@@ -51,81 +51,85 @@ Proof.
   simpl.
   induction 1 using glu_sort_elem_ind; intros;
     simpl_glu_rel; mauto 4.
-  - assert {{ Γ ⊢ A : Sort@s }}.
-    {
-      assert {{ Γ ⊢ Sort@s' : Sort@s }} by mauto 2.
-      assert {{ Γ ⊢ A[Id] ≈ Sort@s' : Sort@s }} by (eapply H4; mauto 3).
-      gen_presup H6.
-      mauto 2.
-    }
-    repeat split.
-    + etransitivity; mauto 3.      
-    + intros.
-      assert {{ Δ ⊢ A[σ] ≈ A'[σ] }} by mauto 3.
-      assert {{ Δ ⊢ A[σ] ≈ A'[σ] : K }} by (eapply H4; mauto 3).
-      assert {{ Δ ⊢ A[σ] ≈ A'0 }} by (etransitivity; mauto 2).
-      gen_presup H10.
-      assert ({{ Δ ⊢ A[σ] : K }} -> {{ Δ ⊢ A[σ] ≈ A'0 : K }}) by (eapply H4; mauto 4).
-      assert {{ Δ ⊢ A[σ] ≈ A'0 : K }} by mauto 2.
-      etransitivity; mauto 3.
-    + intros.
-      assert {{ Δ ⊢ A[σ] ≈ A'[σ] }} by mauto 3.
-      assert {{ Δ ⊢ A[σ] ≈ A'0 }} by (etransitivity; mauto 2).
-      assert {{ Δ ⊢ A[σ] ≈ A'0 : K }} by (eapply H4; mauto 4).
-      gen_presup H11.
-      assert ({{ Δ ⊢ A[σ] : K }} -> {{ Δ ⊢ A[σ] ≈ A'[σ] : K }}) by (eapply H4; mauto 4).
-      assert {{ Δ ⊢ A[σ] ≈ A'[σ] : K }} by mauto 2.
-      etransitivity; mauto 2.
+  split; [eassumption | ].
+  intros.
+  transitivity {{{ A[σ] }}}; mauto 4.
+  
+  (* - assert {{ Γ ⊢ A : Sort@s }}. *)
+  (*   { *)
+  (*     assert {{ Γ ⊢ Sort@s' : Sort@s }} by mauto 2. *)
+  (*     assert {{ Γ ⊢ A[Id] ≈ Sort@s' : Sort@s }} by (eapply H4; mauto 3). *)
+  (*     gen_presup H6. *)
+  (*     mauto 2. *)
+  (*   } *)
+  (*   repeat split. *)
+  (*   + etransitivity; mauto 3.       *)
+  (*   + intros. *)
+  (*     assert {{ Δ ⊢ A[σ] ≈ A'[σ] }} by mauto 3. *)
+  (*     assert {{ Δ ⊢ A[σ] ≈ A'[σ] : K }} by (eapply H4; mauto 3). *)
+  (*     assert {{ Δ ⊢ A[σ] ≈ A'0 }} by (etransitivity; mauto 2). *)
+  (*     gen_presup H10. *)
+  (*     assert ({{ Δ ⊢ A[σ] : K }} -> {{ Δ ⊢ A[σ] ≈ A'0 : K }}) by (eapply H4; mauto 4). *)
+  (*     assert {{ Δ ⊢ A[σ] ≈ A'0 : K }} by mauto 2. *)
+  (*     etransitivity; mauto 3. *)
+  (*   + intros. *)
+  (*     assert {{ Δ ⊢ A[σ] ≈ A'[σ] }} by mauto 3. *)
+  (*     assert {{ Δ ⊢ A[σ] ≈ A'0 }} by (etransitivity; mauto 2). *)
+  (*     assert {{ Δ ⊢ A[σ] ≈ A'0 : K }} by (eapply H4; mauto 4). *)
+  (*     gen_presup H11. *)
+  (*     assert ({{ Δ ⊢ A[σ] : K }} -> {{ Δ ⊢ A[σ] ≈ A'[σ] : K }}) by (eapply H4; mauto 4). *)
+  (*     assert {{ Δ ⊢ A[σ] ≈ A'[σ] : K }} by mauto 2. *)
+  (*     etransitivity; mauto 2. *)
       
-  - econstructor; mauto 2.
-    + assert {{ Γ ⊢ A ≈ A[Id] : Sort@s3 }} by (symmetry; mauto 2).
-      gen_presup H13.
-      assert ({{ Γ ⊢ A[Id] : Sort@s3 }} -> {{ Γ ⊢ A[Id] ≈ A' : Sort@s3 }}) by (eapply H10; mauto 4).
-      assert {{ Γ ⊢ A[Id] ≈ A' : Sort@s3 }} by mauto 2.
-      assert {{ Γ ⊢ A ≈ A' : Sort@s3 }} by (etransitivity; mauto 2).
-      etransitivity; mauto 2.
-    + intros.
-      assert {{ Δ ⊢ A[σ] ≈ A'[σ] }} by mauto 3.
-      assert {{ Δ ⊢ A[σ] ≈ A'0 }} by (etransitivity; mauto 2).
-      split; intros.
-      * assert {{ Δ ⊢ A[σ] ≈ A'[σ] : K }} by (eapply H10; mauto 3).
-        gen_presup H18.
-        assert ({{ Δ ⊢ A[σ] : K }} -> {{ Δ ⊢ A[σ] ≈ A'0 : K }}) by (eapply H10; mauto 3).
-        assert {{ Δ ⊢ A[σ] ≈ A'0 : K }} by mauto 2.
-        etransitivity; mauto 3.
-      * assert {{ Δ ⊢ A[σ] ≈ A'0 : K }} by (eapply H10; mauto 3).
-        gen_presup H18.
-        assert ({{ Δ ⊢ A[σ] : K }} -> {{ Δ ⊢ A[σ] ≈ A'[σ] : K }}) by (eapply H10; mauto 3).
-        assert {{ Δ ⊢ A[σ] ≈ A'[σ] : K }} by mauto 2.
-        etransitivity; mauto 3.
+  (* - econstructor; mauto 2. *)
+  (*   + assert {{ Γ ⊢ A ≈ A[Id] : Sort@s3 }} by (symmetry; mauto 2). *)
+  (*     gen_presup H13. *)
+  (*     assert ({{ Γ ⊢ A[Id] : Sort@s3 }} -> {{ Γ ⊢ A[Id] ≈ A' : Sort@s3 }}) by (eapply H10; mauto 4). *)
+  (*     assert {{ Γ ⊢ A[Id] ≈ A' : Sort@s3 }} by mauto 2. *)
+  (*     assert {{ Γ ⊢ A ≈ A' : Sort@s3 }} by (etransitivity; mauto 2). *)
+  (*     etransitivity; mauto 2. *)
+  (*   + intros. *)
+  (*     assert {{ Δ ⊢ A[σ] ≈ A'[σ] }} by mauto 3. *)
+  (*     assert {{ Δ ⊢ A[σ] ≈ A'0 }} by (etransitivity; mauto 2). *)
+  (*     split; intros. *)
+  (*     * assert {{ Δ ⊢ A[σ] ≈ A'[σ] : K }} by (eapply H10; mauto 3). *)
+  (*       gen_presup H18. *)
+  (*       assert ({{ Δ ⊢ A[σ] : K }} -> {{ Δ ⊢ A[σ] ≈ A'0 : K }}) by (eapply H10; mauto 3). *)
+  (*       assert {{ Δ ⊢ A[σ] ≈ A'0 : K }} by mauto 2. *)
+  (*       etransitivity; mauto 3. *)
+  (*     * assert {{ Δ ⊢ A[σ] ≈ A'0 : K }} by (eapply H10; mauto 3). *)
+  (*       gen_presup H18. *)
+  (*       assert ({{ Δ ⊢ A[σ] : K }} -> {{ Δ ⊢ A[σ] ≈ A'[σ] : K }}) by (eapply H10; mauto 3). *)
+  (*       assert {{ Δ ⊢ A[σ] ≈ A'[σ] : K }} by mauto 2. *)
+  (*       etransitivity; mauto 3. *)
         
-  - repeat split.
-    + assert {{ Γ ⊢ A[Id] : Sort@s }} by mauto 3.
-      assert ({{ Γ ⊢ A[Id] : Sort@s }} -> {{ Γ ⊢ A[Id] ≈ A' : Sort@s }}) by (eapply H4; mauto 3).
-      assert {{ Γ ⊢ A[Id] ≈ A' : Sort@s }} by mauto 2.
-      assert {{ Γ ⊢ A ≈ A[Id] : Sort@s }} by (symmetry; mauto 2).
-      assert {{ Γ ⊢ A ≈ A' : Sort@s }} by (etransitivity; mauto 2).
-      gen_presup H8; eassumption.
-    + intros.
-      assert {{ Δ ⊢ A[σ] ≈ A'[σ] }} by mauto 3.
-      assert {{ Δ ⊢ A[σ] ≈ A'0 }} by (etransitivity; mauto 2).
-      assert {{ Δ ⊢ A[σ] ≈ A'[σ] : K }} by (eapply H4; mauto 3).
-      gen_presup H11.
-      assert ({{ Δ ⊢ A[σ] : K }} -> {{ Δ ⊢ A[σ] ≈ A'0 : K }}) by (eapply H4; mauto 3).
-      assert {{ Δ ⊢ A[σ] ≈ A'0 : K }} by mauto 2.
-      etransitivity; mauto 3.
-    + intros.
-      assert {{ Δ ⊢ A'[σ] ≈ A[σ] }} by (symmetry; mauto 3).
-      assert {{ Δ ⊢ A[σ] ≈ A'0 }} by (etransitivity; mauto 2).
-      assert {{ Δ ⊢ A[σ] ≈ A'0 : K}} by (eapply H4; mauto 3).
-      gen_presup H11.
-      assert ({{ Δ ⊢ A[σ] : K }} -> {{ Δ ⊢ A[σ] ≈ A'[σ] : K }}) by (eapply H4; mauto 3).
-      assert {{ Δ ⊢ A[σ] ≈ A'[σ] : K }} by mauto 2.
-      etransitivity; mauto 3.      
-    + intros.
-      assert {{ Δ ⊢ A'[σ] ≈ A[σ] }} by (symmetry; mauto 3).
-      assert {{ Δ ⊢ A[σ] ≈ A'0 }} by (eapply H5; mauto 2).
-      etransitivity; mauto 2.
+  (* - repeat split. *)
+  (*   + assert {{ Γ ⊢ A[Id] : Sort@s }} by mauto 3. *)
+  (*     assert ({{ Γ ⊢ A[Id] : Sort@s }} -> {{ Γ ⊢ A[Id] ≈ A' : Sort@s }}) by (eapply H4; mauto 3). *)
+  (*     assert {{ Γ ⊢ A[Id] ≈ A' : Sort@s }} by mauto 2. *)
+  (*     assert {{ Γ ⊢ A ≈ A[Id] : Sort@s }} by (symmetry; mauto 2). *)
+  (*     assert {{ Γ ⊢ A ≈ A' : Sort@s }} by (etransitivity; mauto 2). *)
+  (*     gen_presup H8; eassumption. *)
+  (*   + intros. *)
+  (*     assert {{ Δ ⊢ A[σ] ≈ A'[σ] }} by mauto 3. *)
+  (*     assert {{ Δ ⊢ A[σ] ≈ A'0 }} by (etransitivity; mauto 2). *)
+  (*     assert {{ Δ ⊢ A[σ] ≈ A'[σ] : K }} by (eapply H4; mauto 3). *)
+  (*     gen_presup H11. *)
+  (*     assert ({{ Δ ⊢ A[σ] : K }} -> {{ Δ ⊢ A[σ] ≈ A'0 : K }}) by (eapply H4; mauto 3). *)
+  (*     assert {{ Δ ⊢ A[σ] ≈ A'0 : K }} by mauto 2. *)
+  (*     etransitivity; mauto 3. *)
+  (*   + intros. *)
+  (*     assert {{ Δ ⊢ A'[σ] ≈ A[σ] }} by (symmetry; mauto 3). *)
+  (*     assert {{ Δ ⊢ A[σ] ≈ A'0 }} by (etransitivity; mauto 2). *)
+  (*     assert {{ Δ ⊢ A[σ] ≈ A'0 : K}} by (eapply H4; mauto 3). *)
+  (*     gen_presup H11. *)
+  (*     assert ({{ Δ ⊢ A[σ] : K }} -> {{ Δ ⊢ A[σ] ≈ A'[σ] : K }}) by (eapply H4; mauto 3). *)
+  (*     assert {{ Δ ⊢ A[σ] ≈ A'[σ] : K }} by mauto 2. *)
+  (*     etransitivity; mauto 3.       *)
+  (*   + intros. *)
+  (*     assert {{ Δ ⊢ A'[σ] ≈ A[σ] }} by (symmetry; mauto 3). *)
+  (*     assert {{ Δ ⊢ A[σ] ≈ A'0 }} by (eapply H5; mauto 2). *)
+  (*     etransitivity; mauto 2. *)
 Qed.
 
 Add Parametric Morphism {P} (pred_P : PredicativeSig P) s typ_rel exp_rel a (H : glu_sort_elem pred_P s typ_rel exp_rel a) Γ : (typ_rel Γ)
@@ -166,69 +170,70 @@ Proof.
   induction 1 using glu_sort_elem_ind; intros;
     simpl_glu_rel; repeat split; intros; mauto 3.
   
-  - assert {{ Δ ⊢ A[σ] ≈ A'[σ] }} by mauto 3.
-    assert {{ Δ ⊢ A[σ] ≈ A'0 }} by (etransitivity; mauto 2).
-    assert {{ Δ ⊢ A[σ] ≈ A'[σ] : K }} by (eapply H5; mauto 3).
-    gen_presup H13.
-    assert ({{ Δ ⊢ A[σ] : K }} -> {{ Δ ⊢ A[σ] ≈ A'0 : K }}) by (eapply H5; mauto 3).
-    assert {{ Δ ⊢ A[σ] ≈ A'0 : K }} by mauto 2.
-    etransitivity; mauto 3.
-  - assert {{ Δ ⊢ A[σ] ≈ A'[σ] }} by mauto 3.
-    assert {{ Δ ⊢ A[σ] ≈ A'0 }} by (etransitivity; mauto 2).
-    assert {{ Δ ⊢ A[σ] ≈ A'0 : K }} by (eapply H5; mauto 2).
-    gen_presup H13.
-    assert ({{ Δ ⊢ A[σ] : K }} -> {{ Δ ⊢ A[σ] ≈ A'[σ] : K }}) by (eapply H5; mauto 3).
-    assert {{ Δ ⊢ A[σ] ≈ A'[σ] : K }} by mauto 2.
-    etransitivity; mauto 3.
-  (* - assert ({{ Δ ⊢ M[σ] : B }} -> {{ Δ ⊢ M[σ] ≈ M' : B}}) by (eapply H6; mauto 3). *)
-  (*   mauto 2. *)
-  (* - eapply H6; mauto 3. *)
+  (* - assert {{ Δ ⊢ A[σ] ≈ A'[σ] }} by mauto 3. *)
+  (*   assert {{ Δ ⊢ A[σ] ≈ A'0 }} by (etransitivity; mauto 2). *)
+  (*   assert {{ Δ ⊢ A[σ] ≈ A'[σ] : K }} by (eapply H5; mauto 3). *)
+  (*   gen_presup H13. *)
+  (*   assert ({{ Δ ⊢ A[σ] : K }} -> {{ Δ ⊢ A[σ] ≈ A'0 : K }}) by (eapply H5; mauto 3). *)
+  (*   assert {{ Δ ⊢ A[σ] ≈ A'0 : K }} by mauto 2. *)
+  (*   etransitivity; mauto 3. *)
+  (* - assert {{ Δ ⊢ A[σ] ≈ A'[σ] }} by mauto 3. *)
+  (*   assert {{ Δ ⊢ A[σ] ≈ A'0 }} by (etransitivity; mauto 2). *)
+  (*   assert {{ Δ ⊢ A[σ] ≈ A'0 : K }} by (eapply H5; mauto 2). *)
+  (*   gen_presup H13. *)
+  (*   assert ({{ Δ ⊢ A[σ] : K }} -> {{ Δ ⊢ A[σ] ≈ A'[σ] : K }}) by (eapply H5; mauto 3). *)
+  (*   assert {{ Δ ⊢ A[σ] ≈ A'[σ] : K }} by mauto 2. *)
+  (*   etransitivity; mauto 3. *)
+  (* (* - assert ({{ Δ ⊢ M[σ] : B }} -> {{ Δ ⊢ M[σ] ≈ M' : B}}) by (eapply H6; mauto 3). *) *)
+  (* (*   mauto 2. *) *)
+  (* (* - eapply H6; mauto 3. *) *)
   - firstorder.
 
   - econstructor; mauto 3.
-    + assert {{ Γ ⊢ A ≈ A[Id] : Sort@s3 }} by (symmetry; mauto 2).
-      gen_presup H15.
-      assert ({{ Γ ⊢ A[Id] : Sort@s3 }} -> {{ Γ ⊢ A[Id] ≈ A' : Sort@s3 }}) by (eapply H12; mauto 3).
-      assert {{ Γ ⊢ A[Id] ≈ A' : Sort@s3 }} by mauto 2.
-      assert {{ Γ ⊢ A ≈ A' : Sort@s3 }} by (etransitivity; mauto 2).
-      etransitivity; mauto 2.
-    + intros.
-      assert {{ Δ ⊢ A[σ] ≈ A'[σ] }} by mauto 3.
-      assert {{ Δ ⊢ A[σ] ≈ A'0 }} by (etransitivity; mauto 2).
-      split; intros.
-      * assert {{ Δ ⊢ A'[σ] ≈ A[σ] : K }} by (symmetry; eapply H12; mauto 2).
-        gen_presup H20.
-        assert ({{ Δ ⊢ A[σ] : K }} -> {{ Δ ⊢ A[σ] ≈ A'0 : K }}) by (eapply H12; mauto 2).
-        assert {{ Δ ⊢ A[σ] ≈ A'0 : K }} by mauto 2.
-        etransitivity; mauto 2.
-      * assert {{ Δ ⊢ A'0 ≈ A[σ] : K }} by (symmetry; eapply H12; mauto 2).
-        gen_presup H20.
-        assert ({{ Δ ⊢ A[σ] : K }} -> {{ Δ ⊢ A[σ] ≈ A'[σ] : K }}) by (eapply H12; mauto 2).
-        assert {{ Δ ⊢ A[σ] ≈ A'[σ] : K }} by mauto 2.
-        etransitivity; mauto 2.
+    (* + assert {{ Γ ⊢ A ≈ A[Id] : Sort@s3 }} by (symmetry; mauto 2). *)
+    (*   gen_presup H15. *)
+    (*   assert ({{ Γ ⊢ A[Id] : Sort@s3 }} -> {{ Γ ⊢ A[Id] ≈ A' : Sort@s3 }}) by (eapply H12; mauto 3). *)
+    (*   assert {{ Γ ⊢ A[Id] ≈ A' : Sort@s3 }} by mauto 2. *)
+    (*   assert {{ Γ ⊢ A ≈ A' : Sort@s3 }} by (etransitivity; mauto 2). *)
+    (*   etransitivity; mauto 2. *)
+    (* + intros. *)
+    (*   assert {{ Δ ⊢ A[σ] ≈ A'[σ] }} by mauto 3. *)
+    (*   assert {{ Δ ⊢ A[σ] ≈ A'0 }} by (etransitivity; mauto 2). *)
+    (*   split; intros. *)
+    (*   * assert {{ Δ ⊢ A'[σ] ≈ A[σ] : K }} by (symmetry; eapply H12; mauto 2). *)
+    (*     gen_presup H20. *)
+    (*     assert ({{ Δ ⊢ A[σ] : K }} -> {{ Δ ⊢ A[σ] ≈ A'0 : K }}) by (eapply H12; mauto 2). *)
+    (*     assert {{ Δ ⊢ A[σ] ≈ A'0 : K }} by mauto 2. *)
+    (*     etransitivity; mauto 2. *)
+    (*   * assert {{ Δ ⊢ A'0 ≈ A[σ] : K }} by (symmetry; eapply H12; mauto 2). *)
+    (*     gen_presup H20. *)
+    (*     assert ({{ Δ ⊢ A[σ] : K }} -> {{ Δ ⊢ A[σ] ≈ A'[σ] : K }}) by (eapply H12; mauto 2). *)
+    (*     assert {{ Δ ⊢ A[σ] ≈ A'[σ] : K }} by mauto 2. *)
+    (*     etransitivity; mauto 2. *)
       
-  - assert ({{ Γ ⊢ A[Id] : Sort@s }} -> {{ Γ ⊢ A[Id] ≈ A' : Sort@s }}) by (eapply H4; mauto 3).
-    assert {{ Γ ⊢ A[Id] : Sort@s }} by mauto 3.
-    assert {{ Γ ⊢ A[Id] ≈ A' : Sort@s }} by mauto 3.
-    gen_presup H11; eassumption.
-  - assert {{ Δ ⊢ A[σ] ≈ A'[σ] }} by mauto 3.
-    assert {{ Δ ⊢ A[σ] ≈ A'0 }} by (etransitivity; mauto 2).
-    assert {{ Δ ⊢ A'[σ] ≈ A[σ] : K }} by (symmetry; eapply H4; mauto 2).
-    gen_presup H14.
-    assert ({{ Δ ⊢ A[σ] : K }} -> {{ Δ ⊢ A[σ] ≈ A'0 : K }}) by (eapply H4; mauto 2).
-    assert {{ Δ ⊢ A[σ] ≈ A'0 : K }} by mauto 2.
-    etransitivity; mauto 2.
-  - assert {{ Δ ⊢ A[σ] ≈ A'[σ] }} by mauto 3.
-    assert {{ Δ ⊢ A[σ] ≈ A'0 }} by (etransitivity; mauto 2).
-    assert {{ Δ ⊢ A'0 ≈ A[σ] : K }} by (symmetry; eapply H4; mauto 2).
-    gen_presup H14.
-    assert ({{ Δ ⊢ A[σ] : K }} -> {{ Δ ⊢ A[σ] ≈ A'[σ] : K }}) by (eapply H4; mauto 2).
-    assert {{ Δ ⊢ A[σ] ≈ A'[σ] : K }} by mauto 2.
-    etransitivity; mauto 2.
+  (* - assert ({{ Γ ⊢ A[Id] : Sort@s }} -> {{ Γ ⊢ A[Id] ≈ A' : Sort@s }}) by (eapply H4; mauto 3). *)
+  (*   assert {{ Γ ⊢ A[Id] : Sort@s }} by mauto 3. *)
+  (*   assert {{ Γ ⊢ A[Id] ≈ A' : Sort@s }} by mauto 3. *)
+  (*   gen_presup H11; eassumption. *)
+  (* - assert {{ Δ ⊢ A[σ] ≈ A'[σ] }} by mauto 3. *)
+  (*   assert {{ Δ ⊢ A[σ] ≈ A'0 }} by (etransitivity; mauto 2). *)
+  (*   assert {{ Δ ⊢ A'[σ] ≈ A[σ] : K }} by (symmetry; eapply H4; mauto 2). *)
+  (*   gen_presup H14. *)
+  (*   assert ({{ Δ ⊢ A[σ] : K }} -> {{ Δ ⊢ A[σ] ≈ A'0 : K }}) by (eapply H4; mauto 2). *)
+  (*   assert {{ Δ ⊢ A[σ] ≈ A'0 : K }} by mauto 2. *)
+  (*   etransitivity; mauto 2. *)
+  (* - assert {{ Δ ⊢ A[σ] ≈ A'[σ] }} by mauto 3. *)
+  (*   assert {{ Δ ⊢ A[σ] ≈ A'0 }} by (etransitivity; mauto 2). *)
+  (*   assert {{ Δ ⊢ A'0 ≈ A[σ] : K }} by (symmetry; eapply H4; mauto 2). *)
+  (*   gen_presup H14. *)
+  (*   assert ({{ Δ ⊢ A[σ] : K }} -> {{ Δ ⊢ A[σ] ≈ A'[σ] : K }}) by (eapply H4; mauto 2). *)
+  (*   assert {{ Δ ⊢ A[σ] ≈ A'[σ] : K }} by mauto 2. *)
+  (*   etransitivity; mauto 2. *)
     
-  - assert {{ Δ ⊢ A'[σ] ≈ A[σ] }} by (symmetry; mauto 3).
-    assert {{ Δ ⊢ A[σ] ≈ A'0 }} by (eapply H8; mauto 2).
-    etransitivity; mauto 2.
+  - transitivity {{{ A[σ] }}}; mauto 4.
+    (* assert {{ Δ ⊢ A'[σ] ≈ A[σ] }} by (symmetry; mauto 3). *)
+    (* assert {{ Δ ⊢ A[σ] ≈ A'0 }} by (eapply H8; mauto 2). *)
+    (* etransitivity; mauto 2. *)
   - assert {{ Δ ⊢ M[σ] ≈ M' : A[σ] }} by mauto 2.
     eapply wf_exp_eq_conv'; mauto 3.
 Qed.
@@ -250,7 +255,6 @@ Corollary glu_sort_elem_trm_resp_typ_exp_eq {P} (pred_P : PredicativeSig P) : fo
       {{ Γ ⊢ M : A' ® m ∈ exp_rel }}.
 Proof.
   intros.
-  assert {{ Γ ⊢ A ≈ A' : Sort@s }} by mauto 2.
   eapply glu_sort_elem_trm_resp_typ_eq; mauto 2.
 Qed.
 
@@ -274,9 +278,9 @@ Proof.
   induction 1 using glu_sort_elem_ind; intros;
     simpl_glu_rel; mauto 2;
     econstructor; mauto 4.
-  - assert {{ ⊢ Γ, IT ≈ Δ, IT }} by mauto 4.
-    mauto 2.
-  - split; intros; mauto 4.
+  (* - assert {{ ⊢ Γ, IT ≈ Δ, IT }} by mauto 4. *)
+  (*   mauto 2. *)
+  (* - split; intros; mauto 4. *)
 Qed.
 
 Add Parametric Morphism {P} (pred_P : PredicativeSig P) s typ_rel exp_rel a (H : glu_sort_elem pred_P s typ_rel exp_rel a) : typ_rel
@@ -288,16 +292,16 @@ Proof.
 Qed.
 
 
-Lemma glu_sort_elem_trm_resp_ctx_eq_pi_helper {P} (pred_P : PredicativeSig P) : forall {s1 s2} (s : P) (r : Ru P s1 s2 s) IR IP IEL elem_rel OEL Γ M A m Δ,
-  {{ Γ ⊢ M : A ® m ∈ pi_glu_exp_pred s r IR IP IEL elem_rel OEL }} ->
+Lemma glu_sort_elem_trm_resp_ctx_eq_pi_helper {P} (pred_P : PredicativeSig P) : forall {s1 s2 s3} (r : Ru P s1 s2 s3) IR IP IEL elem_rel OEL Γ M A m Δ,
+  {{ Γ ⊢ M : A ® m ∈ pi_glu_exp_pred r IR IP IEL elem_rel OEL }} ->
   {{ ⊢ Γ ≈ Δ }} ->
-  {{ Δ ⊢ M : A ® m ∈ pi_glu_exp_pred s r IR IP IEL elem_rel OEL }}.
+  {{ Δ ⊢ M : A ® m ∈ pi_glu_exp_pred r IR IP IEL elem_rel OEL }}.
 Proof.
   intros.
   inversion_clear H.
   econstructor; mauto 4.
-  assert {{ ⊢ Γ, IT ≈ Δ, IT }} by mauto 4.
-  mauto 2.
+  (* assert {{ ⊢ Γ, IT ≈ Δ, IT }} by mauto 4. *)
+  (* mauto 2. *)
 Qed.
 
 
@@ -312,25 +316,25 @@ Proof.
   induction 1 using glu_sort_elem_ind; intros;
     simpl_glu_rel; mauto 2.
   - repeat split; mauto 3.
-    + assert {{ Δ0 ⊢w σ : Γ }} by mauto 3.
-      eapply H5; mauto 3.
-    + assert {{ Δ0 ⊢w σ : Γ }} by mauto 3.
-      eapply H5; mauto 3.
-    (* + eapply H6; mauto 3. *)
-    (* + eapply H6; mauto 3. *)
+    (* + assert {{ Δ0 ⊢w σ : Γ }} by mauto 3. *)
+    (*   eapply H5; mauto 3. *)
+    (* + assert {{ Δ0 ⊢w σ : Γ }} by mauto 3. *)
+    (*   eapply H5; mauto 3. *)
+    (* (* + eapply H6; mauto 3. *) *)
+    (* (* + eapply H6; mauto 3. *) *)
     + do 2 eexists; split; mauto 4.    
       eapply glu_sort_elem_typ_resp_ctx_eq; mauto 2.
 
   - eapply glu_sort_elem_trm_resp_ctx_eq_pi_helper; mauto.
   - econstructor; mauto 4.
     repeat split; mauto 2; intros.
-    + intros.
-      assert {{ Δ0 ⊢w σ : Γ }} by mauto 3.
-      assert ({{ Δ0 ⊢ A[σ] : K }} -> {{ Δ0 ⊢ A[σ] ≈ A' : K }}) by (eapply H4; mauto 3).
-      mauto 2.
-    + intros.
-      assert {{ Δ0 ⊢w σ : Γ }} by mauto 3.
-      eapply H4; mauto 3.
+    (* + intros. *)
+    (*   assert {{ Δ0 ⊢w σ : Γ }} by mauto 3. *)
+    (*   assert ({{ Δ0 ⊢ A[σ] : K }} -> {{ Δ0 ⊢ A[σ] ≈ A' : K }}) by (eapply H4; mauto 3). *)
+    (*   mauto 2. *)
+    (* + intros. *)
+    (*   assert {{ Δ0 ⊢w σ : Γ }} by mauto 3. *)
+    (*   eapply H4; mauto 3. *)
     + mauto 4.
 Qed.
 
@@ -402,7 +406,7 @@ Proof.
     apply_relation_equivalence.
     assert (rel_mod_app m n m n' (x0 n n' equiv_n_n')) by mauto.
     simplify_evals.
-    rewrite -> H23 in H8.
+    rewrite -> H22 in H8.
     eassumption.    
 Qed.
 
@@ -463,8 +467,8 @@ Proof.
     simpl_glu_rel;
     repeat split; mauto 3.
 
-  - eapply H5; mauto 3.
-  - eapply H5; mauto 3.
+  (* - eapply H5; mauto 3. *)
+  (* - eapply H5; mauto 3. *)
   (* - intros. *)
   (*   assert {{ Γ ⊢ M ≈ M' }} by mauto 4. *)
   (*   assert {{ Δ ⊢ M[σ] ≈ M'[σ] }} by mauto 3. *)
@@ -487,6 +491,8 @@ Proof.
     eapply glu_sort_elem_typ_resp_typ_eq; mauto.
 
   - econstructor; eauto.
+    assert ({{ Γ ⊢ IT : Sort@s1 }} /\ {{ Γ, IT ⊢ OT : Sort@s2 }}) by (gen_presup H9; mauto 2).
+    destruct_conjs.
     match_by_head (@per_sort_elem P) ltac:(fun H => directed invert_per_sort_elem H).
     intros.
     destruct_rel_mod_eval.
@@ -495,23 +501,24 @@ Proof.
     eexists; split; eauto.
     enough {{ Δ ⊢ M[σ] N ≈ M'[σ] N : OT[σ,,N] }} by eauto.
     assert {{ Γ ⊢ M ≈ M' : Π r IT OT }} as Hty by mauto.
-    eassert {{ Δ ⊢ IT[σ] : Sort@_ }} by mauto 3.
+    assert {{ Δ ⊢ IT[σ] : Sort@s1 }} by mauto 3.
+    assert {{ Δ, IT[σ] ⊢ OT[q σ] : Sort@s2 }} by mauto 4.
     eapply wf_exp_eq_sub_cong with (Γ := Δ) in Hty; [| eapply sub_eq_refl; mauto 3].
     autorewrite with mcpts in Hty.
-    eapply wf_exp_eq_app_cong with (N := N) (N' := N) in Hty.  (* try pi_sort_level_tac; [|mauto 2]. *)
+    eapply wf_exp_eq_app_cong with (N := N) (N' := N) in Hty; mauto 2.  (* try pi_sort_level_tac; [|mauto 2]. *)
     (* autorewrite with mcpts in Hty. *)
     assert ({{ Δ ⊢ OT[q σ][Id,,N] ≈ OT[σ,,N] }}) by mauto 4.
     mauto.
-    + eassumption.
-    + assert {{ Δ, IT[σ] ⊢s q σ : Γ, IT }} by mauto 4.
-      eapply wf_conv with (A := {{{ Sort@s2[q σ] }}}); mauto 4.
-    + mauto.
+    (* + eassumption. *)
+    (* + assert {{ Δ, IT[σ] ⊢s q σ : Γ, IT }} by mauto 4. *)
+    (*   eapply wf_conv with (A := {{{ Sort@s2[q σ] }}}); mauto 4. *)
+    (* + mauto. *)
 
-  - intros.
-    assert ({{ Δ ⊢ A[σ] : K }} -> {{ Δ ⊢ A[σ] ≈ A' : K }}) by (eapply H4; mauto 3).
-    mauto 2.    
-  - intros.
-    eapply H4; mauto 3.
+  (* - intros. *)
+  (*   assert ({{ Δ ⊢ A[σ] : K }} -> {{ Δ ⊢ A[σ] ≈ A' : K }}) by (eapply H4; mauto 3). *)
+  (*   mauto 2.     *)
+  (* - intros. *)
+  (*   eapply H4; mauto 3. *)
 
   - intros.
     enough {{ Δ ⊢ M[σ] ≈ M'[σ] : A[σ] }}; mauto 4.
@@ -596,7 +603,7 @@ Proof with mautosolve.
 Qed.
 
 (** *** Morphism instances for [neut_glu_*_pred]s *)
-Add Parametric Morphism {P : PtsSig} (s : P) : (neut_glu_typ_pred s)
+Add Parametric Morphism {P : PtsSig} : (@neut_glu_typ_pred P)
     with signature per_bot ==> eq ==> eq ==> iff as neut_glu_typ_pred_morphism_iff.
 Proof with mautosolve.
   split; intros []; econstructor; intuition;
@@ -604,13 +611,13 @@ Proof with mautosolve.
     functional_read_rewrite_clear; intuition.
 Qed.
 
-Add Parametric Morphism {P : PtsSig} (s : P) : (neut_glu_typ_pred s)
+Add Parametric Morphism {P : PtsSig} : (@neut_glu_typ_pred P)
     with signature per_bot ==> glu_typ_pred_equivalence P as neut_glu_typ_pred_morphism_glu_typ_pred_equivalence.
 Proof with mautosolve.
   split; apply neut_glu_typ_pred_morphism_iff; mauto.
 Qed.
 
-Add Parametric Morphism {P : PtsSig} (s : P) : (neut_glu_exp_pred s)
+Add Parametric Morphism {P : PtsSig} : (@neut_glu_exp_pred P)
     with signature per_bot ==> eq ==> eq ==> eq ==> eq ==> iff as neut_glu_exp_pred_morphism_iff.
 Proof with mautosolve.
   split; intros []; econstructor; intuition;
@@ -619,32 +626,32 @@ Proof with mautosolve.
     match_by_head (@per_bot P) ltac:(fun H => rewrite H in *); eassumption.
 Qed.
 
-Add Parametric Morphism {P : PtsSig} (s : P) : (neut_glu_exp_pred s)
+Add Parametric Morphism {P : PtsSig} : (@neut_glu_exp_pred P)
     with signature per_bot ==> glu_exp_pred_equivalence P as neut_glu_exp_pred_morphism_glu_exp_pred_equivalence.
 Proof with mautosolve.
   split; apply neut_glu_exp_pred_morphism_iff; mauto.
 Qed.
 
 (** *** Morphism instances for [pi_glu_*_pred]s *)
-Add Parametric Morphism {P : PtsSig} {s1 s2} (s : P) (r : Ru P s1 s2 s) IR : (pi_glu_typ_pred s r IR)
+Add Parametric Morphism {P : PtsSig} {s1 s2 s3} (r : Ru P s1 s2 s3) IR : (pi_glu_typ_pred r IR)
     with signature glu_typ_pred_equivalence P ==> glu_exp_pred_equivalence P ==> eq ==> eq ==> eq ==> iff as pi_glu_typ_pred_morphism_iff.
 Proof with mautosolve.
   split; intros []; econstructor; intuition.
 Qed.
 
-Add Parametric Morphism {P : PtsSig} {s1 s2} (s : P) (r : Ru P s1 s2 s) IR : (pi_glu_typ_pred s r IR)
+Add Parametric Morphism {P : PtsSig} {s1 s2 s3} (r : Ru P s1 s2 s3) IR : (pi_glu_typ_pred r IR)
     with signature glu_typ_pred_equivalence P ==> glu_exp_pred_equivalence P ==> eq ==> glu_typ_pred_equivalence P as pi_glu_typ_pred_morphism_glu_typ_pred_equivalence.
 Proof with mautosolve.
   split; intros []; econstructor; intuition.
 Qed.
 
-Add Parametric Morphism {P : PtsSig} {s1 s2} (s : P) (r : Ru P s1 s2 s) IR : (pi_glu_exp_pred s r IR)
+Add Parametric Morphism {P : PtsSig} {s1 s2 s3} (r : Ru P s1 s2 s3) IR : (pi_glu_exp_pred r IR)
     with signature glu_typ_pred_equivalence P ==> glu_exp_pred_equivalence P ==> relation_equivalence ==> eq ==> eq ==> eq ==> eq ==> eq ==> iff as pi_glu_exp_pred_morphism_iff.
 Proof with mautosolve.
   split; intros []; econstructor; intuition.
 Qed.
 
-Add Parametric Morphism {P : PtsSig} {s1 s2} (s : P) (r : Ru P s1 s2 s) IR : (pi_glu_exp_pred s r IR)
+Add Parametric Morphism {P : PtsSig} {s1 s2 s3} (r : Ru P s1 s2 s3) IR : (pi_glu_exp_pred r IR)
     with signature glu_typ_pred_equivalence P ==> glu_exp_pred_equivalence P ==> relation_equivalence ==> eq ==> glu_exp_pred_equivalence P as pi_glu_exp_pred_morphism_glu_exp_pred_equivalence.
 Proof with mautosolve.
   split; intros []; econstructor; intuition.
@@ -687,7 +694,7 @@ Proof.
          assert ((s2 = s3 -> glu_sort_elem pred_P s3 (OP0 m equiv0_m) (OEL0 m equiv0_m) a0) /\
                    (pred_rel pred_P s2 s3 -> glu_sort_elem pred_P s2 (OP0 m equiv0_m) (OEL0 m equiv0_m) a0)) by mauto;
          destruct_conjs;
-         destruct H21;
+         destruct H20;
          [
            assert (glu_sort_elem pred_P s2 (OP0 m equiv0_m) (OEL0 m equiv0_m) a0) by mauto;
            eapply H2; mauto
@@ -711,7 +718,7 @@ Proof.
           assert ((s2 = s3 -> glu_sort_elem pred_P s3 (OP0 n equiv0_n) (OEL0 n equiv0_n) a0) /\
                     (pred_rel pred_P s2 s3 -> glu_sort_elem pred_P s2 (OP0 n equiv0_n) (OEL0 n equiv0_n) a0)) by mauto;
           destruct_conjs;
-          destruct H26;
+          destruct H25;
           [
             assert (glu_sort_elem pred_P s2 (OP0 n equiv0_n) (OEL0 n equiv0_n) a0) by mauto;
             eapply H2; mauto
@@ -783,8 +790,8 @@ Lemma glu_sort_elem_pi_clean_inversion1 {P} (pred_P : PredicativeSig P) : forall
             {{ ⟦ B ⟧ ρ ↦ c ↘ b }} ->
             {{ DG b ∈ glu_sort_elem pred_P s2 ↘ OP c equiv_c ↘ OEl c equiv_c }}) /\
         {{ DF Π r a ρ B ≈ Π r a ρ B ∈ per_sort_elem pred_P s3 ↘ elem_rel }} /\
-        (typ_rel <∙> pi_glu_typ_pred s3 r in_rel IP IEl OP) /\
-        (exp_rel <∙> pi_glu_exp_pred s3 r in_rel IP IEl elem_rel OEl).
+        (typ_rel <∙> pi_glu_typ_pred r in_rel IP IEl OP) /\
+        (exp_rel <∙> pi_glu_exp_pred r in_rel IP IEl elem_rel OEl).
 Proof.
   intros *.
   simpl.
@@ -922,8 +929,8 @@ Lemma glu_sort_elem_pi_clean_inversion2 {P} (pred_P : PredicativeSig P) : forall
         {{ ⟦ B ⟧ ρ ↦ c ↘ b }} ->
         {{ DG b ∈ glu_sort_elem pred_P s2 ↘ OP c equiv_c ↘ OEl c equiv_c }}) /\
       {{ DF Π r a ρ B ≈ Π r a ρ B ∈ per_sort_elem pred_P s3 ↘ elem_rel }} /\
-      (typ_rel <∙> pi_glu_typ_pred s3 r in_rel IP IEl OP) /\
-      (exp_rel <∙> pi_glu_exp_pred s3 r in_rel IP IEl elem_rel OEl).
+      (typ_rel <∙> pi_glu_typ_pred r in_rel IP IEl OP) /\
+      (exp_rel <∙> pi_glu_exp_pred r in_rel IP IEl elem_rel OEl).
 Proof.
   intros *.
   simpl.
@@ -983,8 +990,8 @@ Proof.
     mauto 3.
 
   - repeat split; eauto.
-    + eapply H3; mauto 3.
-    + eapply H3; mauto 3.
+    (* + eapply H3; mauto 3. *)
+    (* + eapply H3; mauto 3. *)
     (* + eapply H4; mauto 3. *)
     (* + eapply H4; mauto 3. *)
     + unfold glu_sort_typ_rec in *.
@@ -1005,31 +1012,31 @@ Proof.
   - simpl_glu_rel.
     invert_per_sort_elem H10.
     econstructor; mauto 3.
-    + eapply H18.
-      pose proof (proj1 (H18 _ _) H17).
+    + eapply H17.
+      pose proof (proj1 (H17 _ _) H16).
       simpl in *.
 
       intros.
       saturate_refl_for in_rel.
-      pose proof (H19 _ _ equiv_n_n') as [].
-      pose proof (H19 _ _ H20) as [].
+      pose proof (H18 _ _ equiv_n_n') as [].
+      pose proof (H18 _ _ H19) as [].
       pose proof (H10 _ _ equiv_n_n') as [].
-      pose proof (H10 _ _ H20) as [].
+      pose proof (H10 _ _ H19) as [].
       simplify_evals.
       econstructor; eauto.
       symmetry.
       etransitivity.
       * symmetry. eassumption.
       * handle_per_sort_elem_irrel.
-        eapply H25.
+        eapply H24.
         eassumption.
     + resp_per_IH.
       destruct_rel_mod_eval.
       handle_per_sort_elem_irrel.
-      pose proof (H9 _ equiv_n _ H23).
-      eapply H29 in H26 as []; eauto.
-      destruct (H16 _ _ _ _ H21 H22 equiv_n) as [? []].
-      destruct (H17 _ _ equiv_n) as [].
+      pose proof (H9 _ equiv_n _ H22).
+      eapply H28 in H27 as []; eauto.
+      destruct (H15 _ _ _ _ H20 H21 equiv_n) as [? []].
+      destruct (H16 _ _ equiv_n) as [].
       simplify_evals.
       eauto.
   
@@ -1042,7 +1049,7 @@ Proof.
     econstructor; unfold neut_glu_typ_pred; mauto 3.
 
     intros.
-    specialize (H9 (length Δ)).    
+    specialize (H1 (length Δ)).    
     destruct_all.
     functional_read_rewrite_clear.
     mauto.
@@ -1202,38 +1209,39 @@ Proof.
     simpl in *;
     destruct_all;
     try solve [bulky_rewrite].
-  - repeat split; intros; [transitivity {{{ Sort@s'[σ] }}}; mauto 2 | |];
-      assert {{ Δ0 ⊢w σ∘σ0 : Γ }} by mauto 2.      
-    + gen_presup H0.
-      assert {{ Δ0 ⊢ A[σ∘σ0] ≈ A[σ][σ0] }} by mauto 3.
-      assert {{ Δ0 ⊢ A[σ∘σ0] ≈ A[σ][σ0] : K }} by (eapply H1; mauto 3).
-      gen_presup H9.
-      assert {{ Δ0 ⊢ A[σ∘σ0] ≈ A' }} by (transitivity {{{ A[σ][σ0] }}}; mauto 3).
-      assert ({{ Δ0 ⊢ A[σ∘σ0] : K }} -> {{ Δ0 ⊢ A[σ∘σ0] ≈ A' : K }}) by (eapply H1; mauto 3).
-      transitivity {{{ A[σ∘σ0] }}}; mauto 3.
-    + gen_presup H0.
-      assert {{ Δ0 ⊢ A[σ∘σ0] ≈ A[σ][σ0] }} by mauto 3.
-      assert {{ Δ0 ⊢ A[σ∘σ0] ≈ A' }} by (transitivity {{{ A[σ][σ0] }}}; mauto 3).
-      assert {{ Δ0 ⊢ A[σ∘σ0] ≈ A' : K }} by (eapply H1; mauto 3).
-      gen_presup H10.
-      assert ({{ Δ0 ⊢ A[σ∘σ0] : K }} -> {{ Δ0 ⊢ A[σ∘σ0] ≈ A[σ][σ0] : K }}) by (eapply H1; mauto 3).
-      transitivity {{{ A[σ∘σ0] }}}; mauto 3.
+  - transitivity {{{ Sort@s'[σ] }}}; mauto 2.
+    (* repeat split; intros; [transitivity {{{ Sort@s'[σ] }}}; mauto 2 | |]; *)
+    (*   assert {{ Δ0 ⊢w σ∘σ0 : Γ }} by mauto 2.       *)
+    (* + gen_presup H0. *)
+    (*   assert {{ Δ0 ⊢ A[σ∘σ0] ≈ A[σ][σ0] }} by mauto 3. *)
+    (*   assert {{ Δ0 ⊢ A[σ∘σ0] ≈ A[σ][σ0] : K }} by (eapply H1; mauto 3). *)
+    (*   gen_presup H9. *)
+    (*   assert {{ Δ0 ⊢ A[σ∘σ0] ≈ A' }} by (transitivity {{{ A[σ][σ0] }}}; mauto 3). *)
+    (*   assert ({{ Δ0 ⊢ A[σ∘σ0] : K }} -> {{ Δ0 ⊢ A[σ∘σ0] ≈ A' : K }}) by (eapply H1; mauto 3). *)
+    (*   transitivity {{{ A[σ∘σ0] }}}; mauto 3. *)
+    (* + gen_presup H0. *)
+    (*   assert {{ Δ0 ⊢ A[σ∘σ0] ≈ A[σ][σ0] }} by mauto 3. *)
+    (*   assert {{ Δ0 ⊢ A[σ∘σ0] ≈ A' }} by (transitivity {{{ A[σ][σ0] }}}; mauto 3). *)
+    (*   assert {{ Δ0 ⊢ A[σ∘σ0] ≈ A' : K }} by (eapply H1; mauto 3). *)
+    (*   gen_presup H10. *)
+    (*   assert ({{ Δ0 ⊢ A[σ∘σ0] : K }} -> {{ Δ0 ⊢ A[σ∘σ0] ≈ A[σ][σ0] : K }}) by (eapply H1; mauto 3). *)
+    (*   transitivity {{{ A[σ∘σ0] }}}; mauto 3. *)
       
   - repeat split; intros; mauto 4.
-    + gen_presup H0.
-      assert {{ Δ0 ⊢ A[σ∘σ0] ≈ A[σ][σ0] }} by mauto 3.
-      assert {{ Δ0 ⊢ A[σ∘σ0] ≈ A[σ][σ0] : K }} by (eapply H3; mauto 3).
-      gen_presup H11.
-      assert {{ Δ0 ⊢ A[σ∘σ0] ≈ A' }} by (transitivity {{{ A[σ][σ0] }}}; mauto 3).
-      assert ({{ Δ0 ⊢ A[σ∘σ0] : K }} -> {{ Δ0 ⊢ A[σ∘σ0] ≈ A' : K }}) by (eapply H3; mauto 3).
-      transitivity {{{ A[σ∘σ0] }}}; mauto 3.
-    + gen_presup H0.
-      assert {{ Δ0 ⊢ A[σ∘σ0] ≈ A[σ][σ0] }} by mauto 3.
-      assert {{ Δ0 ⊢ A[σ∘σ0] ≈ A' }} by (transitivity {{{ A[σ][σ0] }}}; mauto 3).
-      assert {{ Δ0 ⊢ A[σ∘σ0] ≈ A' : K }} by (eapply H3; mauto 3).
-      gen_presup H12.
-      assert ({{ Δ0 ⊢ A[σ∘σ0] : K }} -> {{ Δ0 ⊢ A[σ∘σ0] ≈ A[σ][σ0] : K }}) by (eapply H3; mauto 3).
-      transitivity {{{ A[σ∘σ0] }}}; mauto 3.
+    (* + gen_presup H0. *)
+    (*   assert {{ Δ0 ⊢ A[σ∘σ0] ≈ A[σ][σ0] }} by mauto 3. *)
+    (*   assert {{ Δ0 ⊢ A[σ∘σ0] ≈ A[σ][σ0] : K }} by (eapply H3; mauto 3). *)
+    (*   gen_presup H11. *)
+    (*   assert {{ Δ0 ⊢ A[σ∘σ0] ≈ A' }} by (transitivity {{{ A[σ][σ0] }}}; mauto 3). *)
+    (*   assert ({{ Δ0 ⊢ A[σ∘σ0] : K }} -> {{ Δ0 ⊢ A[σ∘σ0] ≈ A' : K }}) by (eapply H3; mauto 3). *)
+    (*   transitivity {{{ A[σ∘σ0] }}}; mauto 3. *)
+    (* + gen_presup H0. *)
+    (*   assert {{ Δ0 ⊢ A[σ∘σ0] ≈ A[σ][σ0] }} by mauto 3. *)
+    (*   assert {{ Δ0 ⊢ A[σ∘σ0] ≈ A' }} by (transitivity {{{ A[σ][σ0] }}}; mauto 3). *)
+    (*   assert {{ Δ0 ⊢ A[σ∘σ0] ≈ A' : K }} by (eapply H3; mauto 3). *)
+    (*   gen_presup H12. *)
+    (*   assert ({{ Δ0 ⊢ A[σ∘σ0] : K }} -> {{ Δ0 ⊢ A[σ∘σ0] ≈ A[σ][σ0] : K }}) by (eapply H3; mauto 3). *)
+    (*   transitivity {{{ A[σ∘σ0] }}}; mauto 3. *)
     (* + assert {{ Γ ⊢ M }} by mauto 3. *)
     (*   assert {{ Δ0 ⊢ M[σ∘σ0] ≈ M[σ][σ0] }} by mauto 3. *)
     (*   assert {{ Δ0 ⊢ M[σ∘σ0] ≈ M[σ][σ0] : B }} by (eapply H5; mauto 3). *)
@@ -1253,22 +1261,27 @@ Proof.
 
   - destruct H7.
     simpl_glu_rel.
+    assert ({{ Γ ⊢ IT : Sort@s1 }} /\ {{ Γ, IT ⊢ OT : Sort@s2 }}) by (gen_presup H4; mauto 3).
+    destruct_conjs.
+    assert {{ Δ ⊢ (Π r IT OT)[σ] ≈ Π r IT[σ] OT[q σ] }} by mauto 3.
+    assert {{ Δ ⊢ A[σ] ≈ Π r IT[σ] OT[q σ] }} by (transitivity {{{ (Π r IT OT)[σ] }}}; mauto 4).
+    
     econstructor; eauto; try solve [bulky_rewrite]; mauto 4.
-    + repeat split; intros.
-      * assert {{ Γ ⊢ A }} by mauto 2.
-        assert {{ Δ0 ⊢ A[σ∘σ0] ≈ A[σ][σ0] }} by mauto 3.
-        assert {{ Δ0 ⊢ A[σ∘σ0] ≈ A[σ][σ0] : K }} by (eapply H9; mauto 3).
-        gen_presup H17.
-        assert {{ Δ0 ⊢ A[σ∘σ0] ≈ A' }} by (transitivity {{{ A[σ][σ0] }}}; mauto 3).
-        assert ({{ Δ0 ⊢ A[σ∘σ0] : K }} -> {{ Δ0 ⊢ A[σ∘σ0] ≈ A' : K }}) by (eapply H9; mauto 3).
-        transitivity {{{ A[σ∘σ0] }}}; mauto 3.
-      * assert {{ Γ ⊢ A }} by mauto 2.
-        assert {{ Δ0 ⊢ A[σ∘σ0] ≈ A[σ][σ0] }} by mauto 3.
-        assert {{ Δ0 ⊢ A[σ∘σ0] ≈ A' }} by (transitivity {{{ A[σ][σ0] }}}; mauto 3).
-        assert {{ Δ0 ⊢ A[σ∘σ0] ≈ A' : K }} by (eapply H9; mauto 3).
-        gen_presup H18.
-        assert ({{ Δ0 ⊢ A[σ∘σ0] : K }} -> {{ Δ0 ⊢ A[σ∘σ0] ≈ A[σ][σ0] : K }}) by (eapply H9; mauto 3).
-        transitivity {{{ A[σ∘σ0] }}}; mauto 3.      
+    (* + repeat split; intros. *)
+    (*   * assert {{ Γ ⊢ A }} by mauto 2. *)
+    (*     assert {{ Δ0 ⊢ A[σ∘σ0] ≈ A[σ][σ0] }} by mauto 3. *)
+    (*     assert {{ Δ0 ⊢ A[σ∘σ0] ≈ A[σ][σ0] : K }} by (eapply H9; mauto 3). *)
+    (*     gen_presup H17. *)
+    (*     assert {{ Δ0 ⊢ A[σ∘σ0] ≈ A' }} by (transitivity {{{ A[σ][σ0] }}}; mauto 3). *)
+    (*     assert ({{ Δ0 ⊢ A[σ∘σ0] : K }} -> {{ Δ0 ⊢ A[σ∘σ0] ≈ A' : K }}) by (eapply H9; mauto 3). *)
+    (*     transitivity {{{ A[σ∘σ0] }}}; mauto 3. *)
+    (*   * assert {{ Γ ⊢ A }} by mauto 2. *)
+    (*     assert {{ Δ0 ⊢ A[σ∘σ0] ≈ A[σ][σ0] }} by mauto 3. *)
+    (*     assert {{ Δ0 ⊢ A[σ∘σ0] ≈ A' }} by (transitivity {{{ A[σ][σ0] }}}; mauto 3). *)
+    (*     assert {{ Δ0 ⊢ A[σ∘σ0] ≈ A' : K }} by (eapply H9; mauto 3). *)
+    (*     gen_presup H18. *)
+    (*     assert ({{ Δ0 ⊢ A[σ∘σ0] : K }} -> {{ Δ0 ⊢ A[σ∘σ0] ≈ A[σ][σ0] : K }}) by (eapply H9; mauto 3). *)
+    (*     transitivity {{{ A[σ∘σ0] }}}; mauto 3.       *)
     + intros.
       eapply IHglu_sort_elem; eauto.
     + intros.
@@ -1290,7 +1303,7 @@ Proof.
       assert {{ Δ0 ⊢ OT[q σ][σ0,,M] ≈ OT[σ∘σ0,,M] : Sort@s2 }} by mauto.
       
       enough (OP m equiv_m Δ0 {{{ OT[σ∘σ0,,M] }}}) by (eapply glu_sort_elem_typ_resp_typ_eq; mauto 3).
-      eapply H11; mauto.
+      eapply H10; mauto.
       assert {{ Δ0 ⊢ IT[σ∘σ0] ≈ IT[σ][σ0] : Sort@s1[σ∘σ0] }} by mauto.
       assert {{ Δ0 ⊢ IT[σ∘σ0] ≈ IT[σ][σ0] : Sort@s1 }} by mauto 4.
       
@@ -1299,24 +1312,29 @@ Proof.
       
   - destruct H7.
     simpl_glu_rel.
+    assert ({{ Γ ⊢ IT : Sort@s1 }} /\ {{ Γ, IT ⊢ OT : Sort@s2 }}) by (gen_presup H7; mauto 3).
+    destruct_conjs.
+    assert {{ Δ ⊢ (Π r IT OT)[σ] ≈ Π r IT[σ] OT[q σ] }} by mauto 3.
+    assert {{ Δ ⊢ A[σ] ≈ Π r IT[σ] OT[q σ] }} by (transitivity {{{ (Π r IT OT)[σ] }}}; mauto 4).
+    
     econstructor; mauto 4;
       intros;
       saturate_weakening_escape.
-    + split; intros.
-      * assert {{ Γ ⊢ A }} by mauto 2.
-        assert {{ Δ0 ⊢ A[σ∘σ0] ≈ A[σ][σ0] }} by mauto 3.
-        assert {{ Δ0 ⊢ A[σ∘σ0] ≈ A[σ][σ0] : K }} by (eapply H11; mauto 3).
-        gen_presup H20.
-        assert {{ Δ0 ⊢ A[σ∘σ0] ≈ A' }} by (transitivity {{{ A[σ][σ0] }}}; mauto 3).
-        assert ({{ Δ0 ⊢ A[σ∘σ0] : K }} -> {{ Δ0 ⊢ A[σ∘σ0] ≈ A' : K }}) by (eapply H11; mauto 3).
-        transitivity {{{ A[σ∘σ0] }}}; mauto 3.
-      * assert {{ Γ ⊢ A }} by mauto 2.
-        assert {{ Δ0 ⊢ A[σ∘σ0] ≈ A[σ][σ0] }} by mauto 3.
-        assert {{ Δ0 ⊢ A[σ∘σ0] ≈ A' }} by (transitivity {{{ A[σ][σ0] }}}; mauto 3).
-        assert {{ Δ0 ⊢ A[σ∘σ0] ≈ A' : K }} by (eapply H11; mauto 3).
-        gen_presup H21.
-        assert ({{ Δ0 ⊢ A[σ∘σ0] : K }} -> {{ Δ0 ⊢ A[σ∘σ0] ≈ A[σ][σ0] : K }}) by (eapply H11; mauto 3).
-        transitivity {{{ A[σ∘σ0] }}}; mauto 3.
+    (* + split; intros. *)
+    (*   * assert {{ Γ ⊢ A }} by mauto 2. *)
+    (*     assert {{ Δ0 ⊢ A[σ∘σ0] ≈ A[σ][σ0] }} by mauto 3. *)
+    (*     assert {{ Δ0 ⊢ A[σ∘σ0] ≈ A[σ][σ0] : K }} by (eapply H11; mauto 3). *)
+    (*     gen_presup H20. *)
+    (*     assert {{ Δ0 ⊢ A[σ∘σ0] ≈ A' }} by (transitivity {{{ A[σ][σ0] }}}; mauto 3). *)
+    (*     assert ({{ Δ0 ⊢ A[σ∘σ0] : K }} -> {{ Δ0 ⊢ A[σ∘σ0] ≈ A' : K }}) by (eapply H11; mauto 3). *)
+    (*     transitivity {{{ A[σ∘σ0] }}}; mauto 3. *)
+    (*   * assert {{ Γ ⊢ A }} by mauto 2. *)
+    (*     assert {{ Δ0 ⊢ A[σ∘σ0] ≈ A[σ][σ0] }} by mauto 3. *)
+    (*     assert {{ Δ0 ⊢ A[σ∘σ0] ≈ A' }} by (transitivity {{{ A[σ][σ0] }}}; mauto 3). *)
+    (*     assert {{ Δ0 ⊢ A[σ∘σ0] ≈ A' : K }} by (eapply H11; mauto 3). *)
+    (*     gen_presup H21. *)
+    (*     assert ({{ Δ0 ⊢ A[σ∘σ0] : K }} -> {{ Δ0 ⊢ A[σ∘σ0] ≈ A[σ][σ0] : K }}) by (eapply H11; mauto 3). *)
+    (*     transitivity {{{ A[σ∘σ0] }}}; mauto 3. *)
         
     + eapply IHglu_sort_elem; eauto.
     + saturate_glu_info.
@@ -1379,20 +1397,20 @@ Proof.
       
   - split; [mauto 3 |].
     repeat split; intros.
-    + assert {{ Γ ⊢ A }} by mauto 2.
-      assert {{ Δ0 ⊢ A[σ∘σ0] ≈ A[σ][σ0] }} by mauto 3.
-      assert {{ Δ0 ⊢ A[σ∘σ0] ≈ A[σ][σ0] : K }} by (eapply H1; mauto 3).
-      gen_presup H10.
-      assert {{ Δ0 ⊢ A[σ∘σ0] ≈ A' }} by (transitivity {{{ A[σ][σ0] }}}; mauto 3).
-      assert ({{ Δ0 ⊢ A[σ∘σ0] : K }} -> {{ Δ0 ⊢ A[σ∘σ0] ≈ A' : K }}) by (eapply H1; mauto 3).
-      transitivity {{{ A[σ∘σ0] }}}; mauto 3.
-    + assert {{ Γ ⊢ A }} by mauto 2.
-      assert {{ Δ0 ⊢ A[σ∘σ0] ≈ A[σ][σ0] }} by mauto 3.
-      assert {{ Δ0 ⊢ A[σ∘σ0] ≈ A' }} by (transitivity {{{ A[σ][σ0] }}}; mauto 3).
-      assert {{ Δ0 ⊢ A[σ∘σ0] ≈ A' : K }} by (eapply H1; mauto 3).
-      gen_presup H11.
-      assert ({{ Δ0 ⊢ A[σ∘σ0] : K }} -> {{ Δ0 ⊢ A[σ∘σ0] ≈ A[σ][σ0] : K }}) by (eapply H1; mauto 3).
-      transitivity {{{ A[σ∘σ0] }}}; mauto 3.
+    (* + assert {{ Γ ⊢ A }} by mauto 2. *)
+    (*   assert {{ Δ0 ⊢ A[σ∘σ0] ≈ A[σ][σ0] }} by mauto 3. *)
+    (*   assert {{ Δ0 ⊢ A[σ∘σ0] ≈ A[σ][σ0] : K }} by (eapply H1; mauto 3). *)
+    (*   gen_presup H10. *)
+    (*   assert {{ Δ0 ⊢ A[σ∘σ0] ≈ A' }} by (transitivity {{{ A[σ][σ0] }}}; mauto 3). *)
+    (*   assert ({{ Δ0 ⊢ A[σ∘σ0] : K }} -> {{ Δ0 ⊢ A[σ∘σ0] ≈ A' : K }}) by (eapply H1; mauto 3). *)
+    (*   transitivity {{{ A[σ∘σ0] }}}; mauto 3. *)
+    (* + assert {{ Γ ⊢ A }} by mauto 2. *)
+    (*   assert {{ Δ0 ⊢ A[σ∘σ0] ≈ A[σ][σ0] }} by mauto 3. *)
+    (*   assert {{ Δ0 ⊢ A[σ∘σ0] ≈ A' }} by (transitivity {{{ A[σ][σ0] }}}; mauto 3). *)
+    (*   assert {{ Δ0 ⊢ A[σ∘σ0] ≈ A' : K }} by (eapply H1; mauto 3). *)
+    (*   gen_presup H11. *)
+    (*   assert ({{ Δ0 ⊢ A[σ∘σ0] : K }} -> {{ Δ0 ⊢ A[σ∘σ0] ≈ A[σ][σ0] : K }}) by (eapply H1; mauto 3). *)
+    (*   transitivity {{{ A[σ∘σ0] }}}; mauto 3. *)
     + intros; mauto 3.
       transitivity {{{ A[σ∘σ0] }}}; mauto 4.
     
@@ -1400,18 +1418,18 @@ Proof.
     econstructor; repeat split; mauto 3;
       intros;
       saturate_weakening_escape.
-    + assert {{ Δ0 ⊢ A[σ∘σ0] ≈ A[σ][σ0] }} by mauto 3.
-      assert {{ Δ0 ⊢ A[σ∘σ0] ≈ A[σ][σ0] : K }} by (eapply H1; mauto 3).
-      gen_presup H13.
-      assert {{ Δ0 ⊢ A[σ∘σ0] ≈ A' }} by (transitivity {{{ A[σ][σ0] }}}; mauto 3).
-      assert ({{ Δ0 ⊢ A[σ∘σ0] : K }} -> {{ Δ0 ⊢ A[σ∘σ0] ≈ A' : K }}) by (eapply H1; mauto 3).
-      transitivity {{{ A[σ∘σ0] }}}; mauto 3.
-    + assert {{ Δ0 ⊢ A[σ∘σ0] ≈ A[σ][σ0] }} by mauto 3.
-      assert {{ Δ0 ⊢ A[σ∘σ0] ≈ A' }} by (transitivity {{{ A[σ][σ0] }}}; mauto 3).
-      assert {{ Δ0 ⊢ A[σ∘σ0] ≈ A' : K }} by (eapply H1; mauto 3).
-      gen_presup H14.
-      assert ({{ Δ0 ⊢ A[σ∘σ0] : K }} -> {{ Δ0 ⊢ A[σ∘σ0] ≈ A[σ][σ0] : K }}) by (eapply H1; mauto 3).
-      transitivity {{{ A[σ∘σ0] }}}; mauto 3.    
+    (* + assert {{ Δ0 ⊢ A[σ∘σ0] ≈ A[σ][σ0] }} by mauto 3. *)
+    (*   assert {{ Δ0 ⊢ A[σ∘σ0] ≈ A[σ][σ0] : K }} by (eapply H1; mauto 3). *)
+    (*   gen_presup H13. *)
+    (*   assert {{ Δ0 ⊢ A[σ∘σ0] ≈ A' }} by (transitivity {{{ A[σ][σ0] }}}; mauto 3). *)
+    (*   assert ({{ Δ0 ⊢ A[σ∘σ0] : K }} -> {{ Δ0 ⊢ A[σ∘σ0] ≈ A' : K }}) by (eapply H1; mauto 3). *)
+    (*   transitivity {{{ A[σ∘σ0] }}}; mauto 3. *)
+    (* + assert {{ Δ0 ⊢ A[σ∘σ0] ≈ A[σ][σ0] }} by mauto 3. *)
+    (*   assert {{ Δ0 ⊢ A[σ∘σ0] ≈ A' }} by (transitivity {{{ A[σ][σ0] }}}; mauto 3). *)
+    (*   assert {{ Δ0 ⊢ A[σ∘σ0] ≈ A' : K }} by (eapply H1; mauto 3). *)
+    (*   gen_presup H14. *)
+    (*   assert ({{ Δ0 ⊢ A[σ∘σ0] : K }} -> {{ Δ0 ⊢ A[σ∘σ0] ≈ A[σ][σ0] : K }}) by (eapply H1; mauto 3). *)
+    (*   transitivity {{{ A[σ∘σ0] }}}; mauto 3.     *)
     + transitivity {{{ A[σ∘σ0] }}}; mauto 4.      
     + transitivity {{{ M[σ∘σ0] }}}; [symmetry|]; mauto 5.
 Qed.
@@ -1607,17 +1625,17 @@ Proof.
   simpl.
   inversion_clear 1; intros; [| eapply glu_sort_elem_typ_resp_typ_eq; mauto 2];
     simpl_glu_rel; mauto 3.
-  repeat split; mauto 3; intros.
-  - assert {{ Δ ⊢ A[σ] ≈ A'[σ] }} by mauto 3.
-    assert {{ Δ ⊢ A[σ] ≈ A'[σ] : K }} by (eapply H3; mauto 3).
-    gen_presup H8.
-    assert ({{ Δ ⊢ A[σ] : K }} -> {{ Δ ⊢ A[σ] ≈ A'0 : K }}) by (eapply H3; mauto 3).
-    transitivity {{{ A[σ] }}}; mauto 3.
-  - assert {{ Δ ⊢ A[σ] ≈ A'[σ] }} by mauto 3.
-    assert {{ Δ ⊢ A[σ] ≈ A'0 : K }} by (eapply H3; mauto 3).
-    gen_presup H8.
-    assert ({{ Δ ⊢ A[σ] : K }} -> {{ Δ ⊢ A[σ] ≈ A'[σ] : K }}) by (eapply H3; mauto 3).
-    transitivity {{{ A[σ] }}}; mauto 3.
+  (* repeat split; mauto 3; intros. *)
+  (* - assert {{ Δ ⊢ A[σ] ≈ A'[σ] }} by mauto 3. *)
+  (*   assert {{ Δ ⊢ A[σ] ≈ A'[σ] : K }} by (eapply H3; mauto 3). *)
+  (*   gen_presup H8. *)
+  (*   assert ({{ Δ ⊢ A[σ] : K }} -> {{ Δ ⊢ A[σ] ≈ A'0 : K }}) by (eapply H3; mauto 3). *)
+  (*   transitivity {{{ A[σ] }}}; mauto 3. *)
+  (* - assert {{ Δ ⊢ A[σ] ≈ A'[σ] }} by mauto 3. *)
+  (*   assert {{ Δ ⊢ A[σ] ≈ A'0 : K }} by (eapply H3; mauto 3). *)
+  (*   gen_presup H8. *)
+  (*   assert ({{ Δ ⊢ A[σ] : K }} -> {{ Δ ⊢ A[σ] ≈ A'[σ] : K }}) by (eapply H3; mauto 3). *)
+  (*   transitivity {{{ A[σ] }}}; mauto 3. *)
 Qed.
 
 Add Parametric Morphism {P} (pred_P : PredicativeSig P) typ_rel exp_rel a (H : glu_typ_unsorted_elem pred_P typ_rel exp_rel a) Γ : (typ_rel Γ)
@@ -1637,20 +1655,20 @@ Proof.
   inversion_clear 1; intros; [| eapply glu_sort_elem_trm_resp_typ_eq; mauto 3];
     simpl_glu_rel; mauto 3.
   repeat split; mauto 3.
-  - intros.
-    assert {{ Δ ⊢ A[σ] ≈ A'[σ] }} by mauto 3.
-    assert {{ Δ ⊢ A[σ] ≈ A'[σ] : K }} by (eapply H4; mauto 3).
-    gen_presup H11.
-    assert ({{ Δ ⊢ A[σ] : K }} -> {{ Δ ⊢ A[σ] ≈ A'0 : K }}) by (eapply H4; mauto 3).
-    transitivity {{{ A[σ] }}}; mauto 3.
-  - intros.
-    assert {{ Δ ⊢ A[σ] ≈ A'[σ] }} by mauto 3.
-    assert {{ Δ ⊢ A[σ] ≈ A'0 : K }} by (eapply H4; mauto 3).
-    gen_presup H11.
-    assert ({{ Δ ⊢ A[σ] : K }} -> {{ Δ ⊢ A[σ] ≈ A'[σ] : K }}) by (eapply H4; mauto 3).
-    transitivity {{{ A[σ] }}}; mauto 3.
-  (* - eapply H5; mauto 3. *)
-  (* - eapply H5; mauto 3. *)
+  (* - intros. *)
+  (*   assert {{ Δ ⊢ A[σ] ≈ A'[σ] }} by mauto 3. *)
+  (*   assert {{ Δ ⊢ A[σ] ≈ A'[σ] : K }} by (eapply H4; mauto 3). *)
+  (*   gen_presup H11. *)
+  (*   assert ({{ Δ ⊢ A[σ] : K }} -> {{ Δ ⊢ A[σ] ≈ A'0 : K }}) by (eapply H4; mauto 3). *)
+  (*   transitivity {{{ A[σ] }}}; mauto 3. *)
+  (* - intros. *)
+  (*   assert {{ Δ ⊢ A[σ] ≈ A'[σ] }} by mauto 3. *)
+  (*   assert {{ Δ ⊢ A[σ] ≈ A'0 : K }} by (eapply H4; mauto 3). *)
+  (*   gen_presup H11. *)
+  (*   assert ({{ Δ ⊢ A[σ] : K }} -> {{ Δ ⊢ A[σ] ≈ A'[σ] : K }}) by (eapply H4; mauto 3). *)
+  (*   transitivity {{{ A[σ] }}}; mauto 3. *)
+  (* (* - eapply H5; mauto 3. *) *)
+  (* (* - eapply H5; mauto 3. *) *)
   - do 2 eexists; split; mauto 3. 
 Qed.
 
@@ -1673,12 +1691,12 @@ Proof.
   simpl.
   inversion_clear 1; intros; [| eapply glu_sort_elem_typ_resp_ctx_eq; mauto 2];
     simpl_glu_rel; mauto 2.
-  repeat split; mauto 3; intros.
-  - intros.
-    assert ({{ Δ0 ⊢ A[σ] : K }} -> {{ Δ0 ⊢ A[σ] ≈ A' : K }}) by (eapply H3; mauto 3).
-    mauto 2.
-  - intros.
-    eapply H3; mauto 3.
+  (* repeat split; mauto 3; intros. *)
+  (* - intros. *)
+  (*   assert ({{ Δ0 ⊢ A[σ] : K }} -> {{ Δ0 ⊢ A[σ] ≈ A' : K }}) by (eapply H3; mauto 3). *)
+  (*   mauto 2. *)
+  (* - intros. *)
+  (*   eapply H3; mauto 3. *)
 Qed.
 
 Add Parametric Morphism {P} (pred_P : PredicativeSig P) typ_rel exp_rel a (H : glu_typ_unsorted_elem pred_P typ_rel exp_rel a) : typ_rel
@@ -1700,10 +1718,10 @@ Proof.
   inversion_clear 1; intros; [| eapply glu_sort_elem_trm_resp_ctx_eq; mauto 2];
     simpl_glu_rel.
   repeat split; mauto 3.
-  - eapply H4; mauto 3.
-  - eapply H4; mauto 3.
-  (* - eapply H5; mauto 3. *)
-  (* - eapply H5; mauto 3. *)
+  (* - eapply H4; mauto 3. *)
+  (* - eapply H4; mauto 3. *)
+  (* (* - eapply H5; mauto 3. *) *)
+  (* (* - eapply H5; mauto 3. *) *)
   - do 2 eexists; split; mauto 3.
     eapply glu_sort_elem_typ_resp_ctx_eq; mauto 2.
 Qed.
@@ -1797,8 +1815,8 @@ Proof.
   inversion_clear 1; intros; [| eapply glu_sort_elem_trm_resp_exp_eq; mauto 2];
     simpl_glu_rel; mauto 2.
   repeat split; mauto 2.
-  - eapply H4; mauto 3.
-  - eapply H4; mauto 3.
+  (* - eapply H4; mauto 3. *)
+  (* - eapply H4; mauto 3. *)
   (* - intros. *)
   (*   assert {{ Γ ⊢ M ≈ M' }} by mauto 3. *)
   (*   assert {{ Δ ⊢ M[σ] ≈ M'[σ] }} by mauto 3. *)
@@ -1844,12 +1862,12 @@ Proof.
     unfold glu_sort_typ_rec.
     split; intros; destruct_conjs; repeat split; mauto 3.
     unfold glu_sort_typ.
-    + eapply H7; mauto 3.
-    + eapply H7; mauto 3.
+    (* + eapply H7; mauto 3. *)
+    (* + eapply H7; mauto 3. *)
     (* + eapply H8; mauto 3. *)
     (* + eapply H8; mauto 3. *)
-    + eapply H7; mauto 3.
-    + eapply H7; mauto 3.
+    (* + eapply H7; mauto 3. *)
+    (* + eapply H7; mauto 3. *)
     (* + eapply H8; mauto 3. *)
     (* + eapply H8; mauto 3. *)
     + do 2 eexists; split; mauto 3.
@@ -1861,13 +1879,13 @@ Proof.
     unfold sort_glu_exp_pred'.
     unfold glu_sort_typ_rec.
     split; intros; destruct_conjs; repeat split; mauto 3.
-    + eapply H7; mauto 3.
-    + eapply H7; mauto 3.
+    (* + eapply H7; mauto 3. *)
+    (* + eapply H7; mauto 3. *)
     (* + eapply H8; mauto 3. *)
     (* + eapply H8; mauto 3.       *)
     + do 2 eexists; split; mauto 3.
-    + eapply H7; mauto 3.
-    + eapply H7; mauto 3.
+    (* + eapply H7; mauto 3. *)
+    (* + eapply H7; mauto 3. *)
     (* + eapply H8; mauto 3. *)
     (* + eapply H8; mauto 3.       *)
 
@@ -1929,12 +1947,12 @@ Proof.
     unfold glu_sort_typ in *.
     destruct_conjs.
     repeat split; mauto 2.
-    + eapply H5; mauto 3.
-    + eapply H5; mauto 3.
+    (* + eapply H5; mauto 3. *)
+    (* + eapply H5; mauto 3. *)
     (* + eapply H6; mauto 3. *)
     (* + eapply H6; mauto 3. *)
     + do 2 eexists; split; mauto 2.
-      eapply (glu_sort_elem_resp_per_sort_elem pred_P s m m' H2 H7 H6 H8 H9); mauto 2.
+      eapply (glu_sort_elem_resp_per_sort_elem pred_P s m m' H2 H6 H5 H7 H8); mauto 2.
   - invert_per_sort_elem H4.
     split; [econstructor; mauto 2| ].
     intros.
@@ -1945,12 +1963,12 @@ Proof.
     unfold glu_sort_typ in *.
     destruct_conjs.
     repeat split; mauto 2.
-    + eapply H5; mauto 3.
-    + eapply H5; mauto 3.
+    (* + eapply H5; mauto 3. *)
+    (* + eapply H5; mauto 3. *)
     (* + eapply H6; mauto 3. *)
     (* + eapply H6; mauto 3. *)
     + do 2 eexists; split; mauto 2.
-      eapply (glu_sort_elem_resp_per_sort_elem pred_P s m m' H3 H7 H6 H8 H9); mauto 2.
+      eapply (glu_sort_elem_resp_per_sort_elem pred_P s m m' H3 H6 H5 H7 H8); mauto 2.
   - split; [eassumption|].
     intros.
     invert_glu_sort_elem H.
@@ -1961,12 +1979,12 @@ Proof.
     unfold per_sort in H2.
     destruct_conjs.
     repeat split; mauto 2.
-    + eapply H5; mauto 3.    
-    + eapply H5; mauto 3.
+    (* + eapply H5; mauto 3.     *)
+    (* + eapply H5; mauto 3. *)
     (* + eapply H6; mauto 3. *)
     (* + eapply H6; mauto 3.     *)
     + do 2 eexists; split; mauto 2.
-      eapply (glu_sort_elem_resp_per_sort_elem pred_P s0 m m' H2 H7 H6 H8 H9); mauto 2.
+      eapply (glu_sort_elem_resp_per_sort_elem pred_P s0 m m' H2 H6 H5 H7 H8); mauto 2.
   - assert (per_sort pred_P s a a) by mauto.
     assert (per_sort pred_P s0 a a') by mauto.
     assert (per_sort pred_P s a a') by (eapply per_sort_trans'; mauto 2).
@@ -2123,40 +2141,40 @@ Proof.
       destruct_conjs.
       repeat split; mauto 3; intros.
       * transitivity {{{ Sort@s[σ] }}}; mauto 3.
-      * gen_presup H2.
-        assert {{ Δ0 ⊢ A[σ∘σ0] ≈ A[σ][σ0] }} by mauto 4.
-        assert {{ Δ0 ⊢ A[σ∘σ0] ≈ A[σ][σ0] : K }} by (eapply H3; mauto 3).
-        gen_presup H8.
-        assert {{ Δ0 ⊢ A[σ∘σ0] ≈ A' }} by (transitivity {{{ A[σ][σ0] }}}; mauto 3).
-        assert ({{ Δ0 ⊢ A[σ∘σ0] : K }} -> {{ Δ0 ⊢ A[σ∘σ0] ≈ A' : K }}) by (eapply H3; mauto 3).
-        transitivity {{{ A[σ∘σ0] }}}; mauto 3.
-      * gen_presup H2.
-        assert {{ Δ0 ⊢ A[σ∘σ0] ≈ A[σ][σ0] }} by mauto 4.
-        assert {{ Δ0 ⊢ A[σ∘σ0] ≈ A' }} by (transitivity {{{ A[σ][σ0] }}}; mauto 3).
-        assert {{ Δ0 ⊢ A[σ∘σ0] ≈ A' : K }} by (eapply H3; mauto 3).
-        gen_presup H9.
-        assert ({{ Δ0 ⊢ A[σ∘σ0] : K }} -> {{ Δ0 ⊢ A[σ∘σ0] ≈ A[σ][σ0] : K }}) by (eapply H3; mauto 3).
-        transitivity {{{ A[σ∘σ0] }}}; mauto 3.    
+      (* * gen_presup H2. *)
+      (*   assert {{ Δ0 ⊢ A[σ∘σ0] ≈ A[σ][σ0] }} by mauto 4. *)
+      (*   assert {{ Δ0 ⊢ A[σ∘σ0] ≈ A[σ][σ0] : K }} by (eapply H3; mauto 3). *)
+      (*   gen_presup H8. *)
+      (*   assert {{ Δ0 ⊢ A[σ∘σ0] ≈ A' }} by (transitivity {{{ A[σ][σ0] }}}; mauto 3). *)
+      (*   assert ({{ Δ0 ⊢ A[σ∘σ0] : K }} -> {{ Δ0 ⊢ A[σ∘σ0] ≈ A' : K }}) by (eapply H3; mauto 3). *)
+      (*   transitivity {{{ A[σ∘σ0] }}}; mauto 3. *)
+      (* * gen_presup H2. *)
+      (*   assert {{ Δ0 ⊢ A[σ∘σ0] ≈ A[σ][σ0] }} by mauto 4. *)
+      (*   assert {{ Δ0 ⊢ A[σ∘σ0] ≈ A' }} by (transitivity {{{ A[σ][σ0] }}}; mauto 3). *)
+      (*   assert {{ Δ0 ⊢ A[σ∘σ0] ≈ A' : K }} by (eapply H3; mauto 3). *)
+      (*   gen_presup H9. *)
+      (*   assert ({{ Δ0 ⊢ A[σ∘σ0] : K }} -> {{ Δ0 ⊢ A[σ∘σ0] ≈ A[σ][σ0] : K }}) by (eapply H3; mauto 3). *)
+      (*   transitivity {{{ A[σ∘σ0] }}}; mauto 3.     *)
 
     + rewrite H0 in *.
       unfold sort_glu_exp_pred in *.
       unfold glu_sort_typ in *.
       destruct_conjs.
-      repeat split; [mauto 3 | transitivity {{{ Sort@s[σ] }}}; mauto 3 | | |]; intros.
-      * gen_presup H2.
-        assert {{ Δ0 ⊢ A[σ∘σ0] ≈ A[σ][σ0] }} by mauto 4.
-        assert {{ Δ0 ⊢ A[σ∘σ0] ≈ A[σ][σ0] : K }} by (eapply H4; mauto 3).
-        gen_presup H13.
-        assert {{ Δ0 ⊢ A[σ∘σ0] ≈ A' }} by (transitivity {{{ A[σ][σ0] }}}; mauto 3).
-        assert ({{ Δ0 ⊢ A[σ∘σ0] : K }} -> {{ Δ0 ⊢ A[σ∘σ0] ≈ A' : K }}) by (eapply H4; mauto 3).
-        transitivity {{{ A[σ∘σ0] }}}; mauto 3.
-      * gen_presup H2.
-        assert {{ Δ0 ⊢ A[σ∘σ0] ≈ A[σ][σ0] }} by mauto 4.
-        assert {{ Δ0 ⊢ A[σ∘σ0] ≈ A' }} by (transitivity {{{ A[σ][σ0] }}}; mauto 3).
-        assert {{ Δ0 ⊢ A[σ∘σ0] ≈ A' : K }} by (eapply H4; mauto 3).
-        gen_presup H14.
-        assert ({{ Δ0 ⊢ A[σ∘σ0] : K }} -> {{ Δ0 ⊢ A[σ∘σ0] ≈ A[σ][σ0] : K }}) by (eapply H4; mauto 3).
-        transitivity {{{ A[σ∘σ0] }}}; mauto 3.
+      repeat split; [mauto 3 | transitivity {{{ Sort@s[σ] }}}; mauto 3 | ]; intros.
+      (* * gen_presup H2. *)
+      (*   assert {{ Δ0 ⊢ A[σ∘σ0] ≈ A[σ][σ0] }} by mauto 4. *)
+      (*   assert {{ Δ0 ⊢ A[σ∘σ0] ≈ A[σ][σ0] : K }} by (eapply H4; mauto 3). *)
+      (*   gen_presup H13. *)
+      (*   assert {{ Δ0 ⊢ A[σ∘σ0] ≈ A' }} by (transitivity {{{ A[σ][σ0] }}}; mauto 3). *)
+      (*   assert ({{ Δ0 ⊢ A[σ∘σ0] : K }} -> {{ Δ0 ⊢ A[σ∘σ0] ≈ A' : K }}) by (eapply H4; mauto 3). *)
+      (*   transitivity {{{ A[σ∘σ0] }}}; mauto 3. *)
+      (* * gen_presup H2. *)
+      (*   assert {{ Δ0 ⊢ A[σ∘σ0] ≈ A[σ][σ0] }} by mauto 4. *)
+      (*   assert {{ Δ0 ⊢ A[σ∘σ0] ≈ A' }} by (transitivity {{{ A[σ][σ0] }}}; mauto 3). *)
+      (*   assert {{ Δ0 ⊢ A[σ∘σ0] ≈ A' : K }} by (eapply H4; mauto 3). *)
+      (*   gen_presup H14. *)
+      (*   assert ({{ Δ0 ⊢ A[σ∘σ0] : K }} -> {{ Δ0 ⊢ A[σ∘σ0] ≈ A[σ][σ0] : K }}) by (eapply H4; mauto 3). *)
+      (*   transitivity {{{ A[σ∘σ0] }}}; mauto 3. *)
       (* * assert {{ Γ ⊢ M }} by mauto 3. *)
       (*   assert {{ Δ0 ⊢ M[σ∘σ0] ≈ M[σ][σ0] }} by mauto 4. *)
       (*   assert {{ Δ0 ⊢ M[σ∘σ0] ≈ M[σ][σ0] : B }} by (eapply H5; mauto 3). *)
@@ -2172,7 +2190,7 @@ Proof.
       (*   assert ({{ Δ0 ⊢ M[σ∘σ0] : B }} -> {{ Δ0 ⊢ M[σ∘σ0] ≈ M[σ][σ0] : B }}) by (eapply H5; mauto 3). *)
       (*   transitivity {{{ M[σ∘σ0] }}}; mauto 3. *)
       * do 2 eexists; split; mauto 3.
-        eapply (glu_sort_elem_mut_monotone pred_P s m H5 H6 H7 Δ σ Γ); mauto 3.
+        eapply (glu_sort_elem_mut_monotone pred_P s m H4 H5 H6 Δ σ Γ); mauto 3.
   - eapply glu_sort_elem_mut_monotone; eassumption.
 Qed.
 
