mechanization/theories/Core/Syntactic/CoreInversions.v
@@ -197,3 +197,4 @@ Qed.
 
 #[export]
 Hint Resolve wf_sub_extend_inversion : mcpts.
+    
